src/iopt/iSimTrace.v
@@ -1,0 +1,492 @@
+From sflib Require Import sflib.
+From Paco Require Import paco.
+
+From PromisingLib Require Import Axioms.
+From PromisingLib Require Import Basic.
+From PromisingLib Require Import Language.
+
+Require Import Event.
+Require Import Time.
+Require Import View.
+Require Import Cell.
+Require Import Memory.
+Require Import TView.
+Require Import Local.
+Require Import Thread.
+Require Import Configuration.
+
+Require Import FulfillStep.
+
+Require Import SimMemory.
+Require Import SimPromises.
+Require Import SimLocal.
+Require Import SimThread.
+Require Import iCompatibility.
+
+Require Import ITreeLang.
+
+Set Implicit Arguments.
+
+
+Definition lang_steps_failure [lang] (st1: Language.state lang): Prop :=
+  exists st2 st3,
+    <<STEPS: rtc ((Language.step lang) ProgramEvent.silent) st1 st2>> /\
+    <<FAILURE: (Language.step lang) ProgramEvent.failure st2 st3>>.
+
+Lemma rtc_lang_tau_step_rtc_thread_tau_step lang
+      st1 st2 lc sc mem
+      (STEP: rtc ((Language.step lang) ProgramEvent.silent) st1 st2):
+  rtc (@Thread.tau_step lang) (Thread.mk lang st1 lc sc mem) (Thread.mk lang st2 lc sc mem).
+Proof.
+  induction STEP.
+  - econs 1.
+  - econs 2; eauto. econs.
+    + econs. econs 2. econs; [|econs 1]; eauto.
+    + ss.
+Qed.
+
+
+Definition SIM_TRACE :=
+  forall R_src R_tgt (sim_val:SIM_VAL R_src R_tgt)
+         (st1_src:(Language.state (lang R_src)))
+         (st1_tgt:(Language.state (lang R_tgt))), Prop.
+
+Definition _sim_trace
+           (sim_trace:SIM_TRACE)
+           R_src R_tgt
+           (sim_val:SIM_VAL R_src R_tgt)
+           (st1_src:(Language.state (lang R_src)))
+           (st1_tgt:(Language.state (lang R_tgt))): Prop :=
+  <<TERMINAL:
+    forall (TERMINAL_TGT: (Language.is_terminal (lang R_tgt)) st1_tgt),
+      <<FAILURE: lang_steps_failure st1_src>> \/
+      exists st2_src,
+        <<STEPS: rtc ((Language.step (lang R_src)) ProgramEvent.silent) st1_src st2_src>> /\
+        <<TERMINAL_SRC: (Language.is_terminal (lang R_src)) st2_src>> /\
+        <<TERMINAL: sim_terminal sim_val st2_src st1_tgt>> >> /\
+  <<STEP:
+    forall e_tgt st3_tgt
+      (STEP_TGT: (Language.step (lang R_tgt)) e_tgt st1_tgt st3_tgt),
+      <<FAILURE: lang_steps_failure st1_src>> \/
+      exists e_src st2_src st3_src,
+        <<EVT: ProgramEvent.ord e_src e_tgt>> /\
+        <<STEPS: rtc ((Language.step (lang R_src)) ProgramEvent.silent) st1_src st2_src>> /\
+        <<STEP_SRC: ILang.opt_step e_src st2_src st3_src>> /\
+        <<SIM: sim_trace _ _ sim_val st3_src st3_tgt>> >>.
+
+Lemma _sim_trace_mon: monotone5 _sim_trace.
+Proof.
+  ii. unfold _sim_trace in *. des; splits; ss.
+  i. exploit STEP; eauto. i. des; eauto.
+  right. esplits; eauto.
+Qed.
+Hint Resolve _sim_trace_mon: paco.
+
+Definition sim_trace: SIM_TRACE := paco5 _sim_trace bot5.
+(* Definition sim_trace: SIM_TRACE := paco5 _sim_trace sim_itree. *)
+
+Lemma sim_trace_sim_thread R_src R_tgt
+      sim_val
+      st1_src lc1_src sc1_src mem1_src
+      st1_tgt lc1_tgt sc1_tgt mem1_tgt
+      (SIM: sim_trace sim_val st1_src st1_tgt)
+      (LOCAL: sim_local SimPromises.bot lc1_src lc1_tgt):
+  @sim_thread
+    (lang R_src) (lang R_tgt)
+    (sim_terminal sim_val)
+    st1_src lc1_src sc1_src mem1_src
+    st1_tgt lc1_tgt sc1_tgt mem1_tgt.
+Proof.
+  revert_until sim_val. pcofix CIH. i.
+  generalize SIM. i. punfold SIM0. unfold _sim_trace in SIM0. des.
+  pfold. ii. splits.
+  - i. exploit TERMINAL; eauto. i. des.
+    + left.
+      unfold lang_steps_failure, Thread.steps_failure in *. des.
+      exploit rtc_lang_tau_step_rtc_thread_tau_step; try exact STEPS. i.
+      esplits; eauto.
+      hexploit sim_local_promise_consistent; eauto. i. des.
+      econs 2. econs; eauto.
+    + right.
+      exploit rtc_lang_tau_step_rtc_thread_tau_step; eauto. i.
+      esplits; eauto.
+  - i. right.
+    exploit sim_local_memory_bot; eauto. i.
+    esplits; eauto.
+  - ii. inv STEP_TGT; inv STEP0; [|inv LOCAL0].
+    + right.
+      exploit sim_local_promise_bot; eauto. i. des.
+      esplits; (try exact SC); eauto; ss.
+      econs 2. econs 1. econs; eauto.
+    + exploit STEP; eauto. i. des.
+      * left.
+        unfold lang_steps_failure, Thread.steps_failure in *. des.
+        exploit rtc_lang_tau_step_rtc_thread_tau_step; try exact STEPS. i.
+        esplits; eauto.
+        hexploit sim_local_promise_consistent; eauto. i. des.
+        econs 2. econs; eauto.
+      * right.
+        inv SIM0; [|done].
+        inv EVT. dependent destruction STEP_SRC.
+        { esplits;
+            (try by apply rtc_lang_tau_step_rtc_thread_tau_step; eauto);
+            (try exact SC);
+            eauto; ss.
+          econs 1.
+        }
+        { esplits;
+            (try by apply rtc_lang_tau_step_rtc_thread_tau_step; eauto);
+            (try exact SC);
+            eauto; ss.
+          econs 2. econs 2. econs; [|econs 1]; eauto.
+        }
+    + exploit STEP; eauto. i. des.
+      { left.
+        unfold lang_steps_failure, Thread.steps_failure in *. des.
+        exploit rtc_lang_tau_step_rtc_thread_tau_step; try exact STEPS. i.
+        esplits; eauto.
+        hexploit sim_local_promise_consistent; eauto. i. des.
+        econs 2. econs; eauto. }
+      right.
+      inv SIM0; ss.
+      inv EVT. dependent destruction STEP_SRC.
+      exploit sim_local_read; eauto. i. des.
+      esplits;
+        (try by apply rtc_lang_tau_step_rtc_thread_tau_step; eauto);
+        (try exact SC).
+      * ss.
+      * econs 2. econs 2. econs; [|econs 2]; eauto.
+      * ss.
+      * ss.
+      * right. apply CIH; auto.
+    + exploit STEP; eauto. i. des.
+      { left.
+        unfold lang_steps_failure, Thread.steps_failure in *. des.
+        exploit rtc_lang_tau_step_rtc_thread_tau_step; try exact STEPS. i.
+        esplits; eauto.
+        hexploit sim_local_promise_consistent; eauto. i. des.
+        econs 2. econs; eauto. }
+      right.
+      inv SIM0; [|done].
+      inv EVT. dependent destruction STEP_SRC.
+      hexploit sim_local_write_bot;
+        (try exact LOCAL);
+        (try exact SC);
+        eauto; try refl; try by viewtac. i. des.
+      esplits;
+        (try by apply rtc_lang_tau_step_rtc_thread_tau_step; eauto);
+        (try exact SC).
+      * ss.
+      * econs 2. econs 2. econs; [|econs 3]; eauto.
+      * ss.
+      * ss.
+      * ss.
+      * right. apply CIH; auto.
+    + exploit STEP; eauto. i. des.
+      { left.
+        unfold lang_steps_failure, Thread.steps_failure in *. des.
+        exploit rtc_lang_tau_step_rtc_thread_tau_step; try exact STEPS. i.
+        esplits; eauto.
+        hexploit sim_local_promise_consistent; eauto. i. des.
+        econs 2. econs; eauto. }
+      right.
+      inv SIM0; [|done].
+      inv EVT. dependent destruction STEP_SRC.
+      exploit Local.read_step_future; eauto. i. des.
+      exploit sim_local_read; eauto; try refl. i. des.
+      exploit Local.read_step_future; eauto. i. des.
+      hexploit sim_local_write_bot;
+        (try exact LOCAL0);
+        (try exact SC);
+        eauto; try refl; try by viewtac. i. des.
+      esplits;
+        (try by apply rtc_lang_tau_step_rtc_thread_tau_step; eauto);
+        (try exact SC).
+      * ss.
+      * econs 2. econs 2. econs; [|econs 4]; eauto.
+      * ss.
+      * ss.
+      * ss.
+      * right. apply CIH; auto.
+    + exploit STEP; eauto. i. des.
+      { left.
+        unfold lang_steps_failure, Thread.steps_failure in *. des.
+        exploit rtc_lang_tau_step_rtc_thread_tau_step; try exact STEPS. i.
+        esplits; eauto.
+        hexploit sim_local_promise_consistent; eauto. i. des.
+        econs 2. econs; eauto. }
+      right.
+      inv SIM0; [|done].
+      inv EVT. dependent destruction STEP_SRC.
+      exploit sim_local_fence;
+        (try exact LOCAL);
+        (try exact SC);
+        eauto; try refl. i. des.
+      esplits;
+        (try by apply rtc_lang_tau_step_rtc_thread_tau_step; eauto);
+        (try exact SC).
+      * ss.
+      * econs 2. econs 2. econs; [|econs 5]; eauto.
+      * ss.
+      * ss.
+      * ss.
+      * right. apply CIH; auto.
+    + exploit STEP; eauto. i. des.
+      { left.
+        unfold lang_steps_failure, Thread.steps_failure in *. des.
+        exploit rtc_lang_tau_step_rtc_thread_tau_step; try exact STEPS. i.
+        esplits; eauto.
+        hexploit sim_local_promise_consistent; eauto. i. des.
+        econs 2. econs; eauto. }
+      right.
+      inv SIM0; [|done].
+      inv EVT. dependent destruction STEP_SRC.
+      exploit sim_local_fence;
+        (try exact LOCAL);
+        (try exact SC);
+        eauto; try refl. i. des.
+      esplits;
+        (try by apply rtc_lang_tau_step_rtc_thread_tau_step; eauto);
+        (try exact SC).
+      * ss.
+      * econs 2. econs 2.
+        econs; [|econs 6]; eauto.
+      * ss.
+      * ss.
+      * ss.
+      * right. apply CIH; auto.
+    + exploit STEP; eauto. i. des.
+      { left.
+        unfold lang_steps_failure, Thread.steps_failure in *. des.
+        exploit rtc_lang_tau_step_rtc_thread_tau_step; try exact STEPS. i.
+        esplits; eauto.
+        hexploit sim_local_promise_consistent; eauto. i. des.
+        econs 2. econs; eauto. }
+      left.
+      inv SIM0; [|done].
+      inv EVT. dependent destruction STEP_SRC.
+      exploit sim_local_failure;
+        (try exact LOCAL);
+        eauto. i. des.
+      unfold Thread.steps_failure.
+      esplits;
+        (try by apply rtc_lang_tau_step_rtc_thread_tau_step; eauto).
+      econs 2. econs; [|econs 7]; eauto.
+Qed.
+
+Lemma sim_trace_sim_itree R_src R_tgt
+      (sim_val:SIM_VAL R_src R_tgt)
+      itr_src
+      itr_tgt
+      (SIM: sim_trace sim_val itr_src itr_tgt):
+  sim_itree sim_val
+            itr_src
+            itr_tgt.
+Proof.
+  ii. apply sim_trace_sim_thread; auto.
+Qed.
+
+Lemma sim_trace_sim_ktree R_src0 R_tgt0 R_src1 R_tgt1
+      (sim_val1: SIM_VAL R_src0 R_tgt0) (sim_val2:SIM_VAL R_src1 R_tgt1)
+      ktr_src
+      ktr_tgt
+      (SIM: forall r_src r_tgt
+                   (SIM_VAL1: sim_val1 r_src r_tgt),
+          sim_trace sim_val2 (ktr_src r_src) (ktr_tgt r_tgt)):
+  sim_ktree sim_val1
+            ktr_src
+            ktr_tgt
+            sim_val2.
+Proof.
+  ii. apply sim_trace_sim_thread; auto.
+Qed.
+
+Lemma sim_trace_ret R_src R_tgt
+      (sim_val:SIM_VAL R_src R_tgt)
+      r_src r_tgt
+      (RET: sim_val r_src r_tgt):
+  sim_trace sim_val
+            (Ret r_src)
+            (Ret r_tgt).
+Proof.
+  pfold. unfold _sim_trace. splits.
+  - i. right. esplits; eauto.
+    + econs; eauto.
+    + econs; eauto.
+  - i. inv STEP_TGT.
+Qed.
+
+
+(* instr *)
+
+Lemma sim_trace_trigger R
+      (i_src i_tgt: MemE.t R)
+      (ORD: MemE.ord i_src i_tgt):
+  sim_trace eq
+            (ITree.trigger i_src)
+            (ITree.trigger i_tgt).
+Proof.
+  unfold ITree.trigger.
+  pfold. unfold _sim_trace. splits.
+  { i. inv TERMINAL_TGT. apply f_equal with (f:=observe) in H; ss. }
+  i. ss. dependent destruction ORD; dependent destruction STEP_TGT.
+  - right. esplits; eauto.
+    + econs; eauto.
+    + econs 2. econs. econs.
+    + left. apply sim_trace_ret. ss.
+  - right. esplits; eauto.
+    + econs; eauto.
+    + econs 2. econs. econs.
+    + left. apply sim_trace_ret. ss.
+  - right. esplits; eauto.
+    + econs; eauto.
+    + econs 2. econs; eauto.
+    + left. apply sim_trace_ret. ss.
+  - right. esplits; eauto.
+    + econs. eauto.
+    + econs 2. econs; eauto.
+    + left. apply sim_trace_ret. ss.
+  - right. esplits; eauto.
+    + econs; eauto.
+    + econs 2. econs. ss.
+    + left. apply sim_trace_ret. ss.
+  - right. esplits; eauto.
+    + econs; eauto.
+    + econs 2. econs. ss.
+    + left. apply sim_trace_ret. ss.
+  - right. esplits; eauto.
+    + econs; eauto.
+    + econs 2. econs. ss.
+    + left. apply sim_trace_ret. ss.
+  - right. esplits; eauto.
+    + econs; eauto.
+    + econs 2. econs. ss.
+    + left. apply sim_trace_ret. ss.
+Qed.
+
+Lemma sim_trace_choose r:
+  sim_trace eq
+            (ITree.trigger MemE.choose)
+            (Ret r).
+Proof.
+  unfold ITree.trigger.
+  pfold. unfold _sim_trace. splits.
+  { i. right. esplits.
+    { econs 2; eauto. econs; eauto. }
+    { econs; eauto. }
+    { econs; try refl. }
+  }
+  i. ss. inv STEP_TGT.
+Qed.
+
+Lemma eutt_sim_trace R_src R_tgt
+      (sim_val: SIM_VAL R_src R_tgt)
+      (itr_src: itree MemE.t R_src) (itr_tgt: itree MemE.t R_tgt)
+      (EUTT: eutt sim_val itr_src itr_tgt)
+  :
+    sim_trace sim_val itr_src itr_tgt.
+Proof.
+  revert R_src R_tgt sim_val itr_src itr_tgt EUTT. pcofix CIH.
+  i. punfold EUTT. unfold eqit_ in EUTT.
+  replace itr_src with (go (observe itr_src)).
+  2:{ apply bisim_is_eq. symmetry. apply itree_eta. }
+  replace itr_tgt with (go (observe itr_tgt)).
+  2:{ apply bisim_is_eq. symmetry. apply itree_eta. }
+  revert EUTT.
+  generalize (observe itr_src) as itr_src'.
+  generalize (observe itr_tgt) as itr_tgt'. clear itr_src itr_tgt. i.
+  induction EUTT.
+  - pfold. econs.
+    2:{ ii. inv STEP_TGT. }
+    ii. right. esplits; eauto.
+    { econs; eauto. }
+    { econs; eauto. }
+  - pclearbot. pfold. econs.
+    { ii. inv TERMINAL_TGT. apply f_equal with (f:=observe) in H; ss. }
+    ii. ss. dependent destruction STEP_TGT. right.
+    esplits; eauto.
+    { econs. }
+    econs 2. econs; eauto.
+  - pclearbot. pfold. econs.
+    { ii. inv TERMINAL_TGT. apply f_equal with (f:=observe) in H; ss. }
+    ii. ss. right.
+    dependent destruction STEP_TGT.
+    + esplits; [econs; refl|eauto|econs 2|right; apply CIH; eauto]; econs; eauto.
+    + esplits; [econs; refl|eauto|econs 2|right; apply CIH; eauto]; econs; eauto.
+    + esplits; [econs; refl|eauto|econs 2|right; apply CIH; eauto]; econs; eauto.
+    + esplits; [econs; refl|eauto|econs 2|right; apply CIH; eauto]; econs; eauto.
+    + esplits; [econs; refl|eauto|econs 2|right; apply CIH; eauto]; econs; eauto.
+    + esplits; [econs; refl|eauto|econs 2|right; apply CIH; eauto]; econs; eauto.
+    + esplits; [econs; refl|eauto|econs 2|right; apply CIH; eauto]; econs; eauto.
+    + esplits; [econs; refl|eauto|econs 2|right; apply CIH; eauto]; econs; eauto.
+  - admit.
+  - pfold. econs.
+    { ii. inv TERMINAL_TGT. apply f_equal with (f:=observe) in H; ss. }
+    ii. ss. right.
+    dependent destruction STEP_TGT.
+    esplits; [econs; refl|eauto|econs 1|]. right. eauto.
+Admitted.
+
+Lemma sim_trace_refl R (itr: itree MemE.t R):
+  sim_trace eq itr itr.
+Proof.
+  eapply eutt_sim_trace. refl.
+Qed.
+
+Lemma sim_itree_refl R (itr: itree MemE.t R):
+  sim_itree eq itr itr.
+Proof.
+  eapply sim_trace_sim_itree.
+  eapply sim_trace_refl.
+Qed.
+
+
+(* replacing abort with arbitrary instructions *)
+
+Lemma sim_trace_replace_abort R (itr: itree MemE.t R):
+  sim_trace bot2
+            (ITree.trigger MemE.abort)
+            itr.
+Proof.
+  pfold. unfold _sim_trace. splits; i.
+  - left.
+    unfold lang_steps_failure. esplits; eauto.
+    econs. ss.
+  - left.
+    unfold lang_steps_failure. esplits; eauto.
+    econs. ss.
+Qed.
+
+Lemma sim_itree_replace_abort R (itr: itree MemE.t R):
+  sim_itree bot2 (ITree.trigger MemE.abort) itr.
+Proof.
+  apply sim_trace_sim_itree. i.
+  apply sim_trace_replace_abort; ss.
+Qed.
+
+
+(* eliminating instructions after abort *)
+
+Lemma sim_trace_elim_after_abort R (k: ktree MemE.t _ R):
+  sim_trace bot2
+            (ITree.trigger MemE.abort >>= k)
+            (ITree.trigger MemE.abort).
+Proof.
+  replace (ITree.trigger MemE.abort >>= k) with
+      (Vis MemE.abort (fun r => k r)).
+  2:{ unfold ITree.trigger. grind. repeat f_equal. extensionality u. grind. }
+  pfold. unfold _sim_trace. splits; i.
+  - inv TERMINAL_TGT. apply f_equal with (f:=observe) in H; ss.
+  - left.
+    unfold lang_steps_failure. esplits; eauto.
+    econs. econs.
+Qed.
+
+Lemma sim_itree_elim_after_abort R (k: ktree MemE.t _ R):
+  sim_itree bot2
+            (ITree.trigger MemE.abort >>= k)
+            (ITree.trigger MemE.abort).
+Proof.
+  apply sim_trace_sim_itree.
+  apply sim_trace_elim_after_abort; ss.
+Qed.
